src/SSmtyP.v
@@ -20,24 +20,41 @@ Fixpoint rcd_cons_ty (rcd : list (id * ty)) (retty : ty) : ty :=
     end. 
 *)
 
-Fixpoint rcd_field_ty (rcd: list (id * ty)) (field : id) : option ty :=
-    match rcd with
-    | nil => None
-    | (i, ret)::t  => if (eq_id_dec i field) 
-                        then Some ret 
-                        else rcd_field_ty t field
-    end.
+Definition rcd_field_ty (rcd: ty) (h : only_rcd rcd) (h' : wf_ty rcd) (field : id) : option ty.
+remember rcd as r.
+generalize dependent h'. generalize dependent field. generalize dependent Heqr. generalize dependent rcd.
+induction h; intros. apply None.
+destruct (eq_id_dec i field) eqn:h2.
+apply (Some T).
+apply (IHh T' eq_refl field).
+inversion h'; subst; eauto.
+Defined.
+
+Theorem rcd_field_ty_well_formed:
+    forall rcd h h' i T,
+        rcd_field_ty rcd h h' i = Some T->
+        wf_ty T.
+    intros rcd h.
+    induction h; intros; eauto.
+    inversion H.
+    cbn in H. destruct (eq_id_dec i i0); subst; eauto.
+    inversion H; subst; eauto.
+    inversion h'; subst; eauto.
+Qed.
 
 
 
-Inductive has_type : Context ty -> tm -> ty -> Prop :=
+
+
+Inductive has_type : Context (type := {x : ty | wf_ty x}) -> tm -> ty -> Prop :=
 | ht_none : 
     forall ctx,
         has_type ctx tnone TNone
 | ht_rcd :
     forall ctx i t0 t1 T T',
-        has_type t0 T ->
-        has_type t1 T' ->
+        has_type ctx t0 T ->
+        has_type ctx t1 T' ->
+        only_rcd T' ->
         has_type ctx (trcons i t0 t1) (TRcons i T T')
 | ht_if : 
     forall ctx crit tb fb T,
@@ -45,11 +62,11 @@ Inductive has_type : Context ty -> tm -> ty -> Prop :=
     has_type ctx tb T ->
     has_type ctx fb T ->
     has_type ctx (tif crit tb fb) T
-| ht_var: forall ctx T i,
-    byContext ctx i = T ->
+| ht_var: forall ctx T i (h: wf_ty T),
+    byContext ctx i = Some (exist _ T h) ->
     has_type ctx (tvar i) T
-| ht_zero : forall ctx,
-    has_type ctx tzero TNat
+| ht_int : forall ctx n,
+    has_type ctx (tint n) TNat
 | ht_suc : forall ctx t,
     has_type ctx t TNat ->
     has_type ctx (tsuc t) TNat
@@ -59,36 +76,36 @@ Inductive has_type : Context ty -> tm -> ty -> Prop :=
 | ht_ngt : forall ctx t0 t1,
     has_type ctx t0 TNat ->
     has_type ctx t1 TNat ->
-    has_type ctx (ngt t0 t1) TBool
+    has_type ctx (tngt t0 t1) TBool
 | ht_nlt : forall ctx t0 t1,
     has_type ctx t0 TNat ->
     has_type ctx t1 TNat ->
-    has_type ctx (nlt t0 t1) TBool
+    has_type ctx (tnlt t0 t1) TBool
 | ht_neq : forall ctx t0 t1,
     has_type ctx t0 TNat ->
     has_type ctx t1 TNat ->
-    has_type ctx (neq t0 t1) TBool
-| ht_neq : forall ctx t0 t1,
-    has_type ctx t0 TNat ->
-    has_type ctx t1 TNat ->
-    has_type ctx (neq t0 t1) TBool
+    has_type ctx (tneq t0 t1) TBool
+
 | ht_chr : forall ctx n,
     has_type ctx (tchr n) TChr
 | ht_ceq : forall ctx t0 t1,
     has_type ctx t0 TChr ->
     has_type ctx t1 TChr ->
-    has_type ctx (ceq t0 t1) TBool
-| ht_fun : forall ctx i T body TO,
-    has_type (update i T ctx) body TO ->
-    has_type ctx (tfun i T body) (TFun T TO)
+    has_type ctx (tceq t0 t1) TBool
+| ht_fun : forall ctx i T body TO (h: wf_ty T),
+    has_type (update i (exist _ T h) ctx) body TO ->
+    has_type ctx (tfun i T h body) (TFun T TO)
 | ht_app : forall ctx t0 t1 T0 T1,
     has_type ctx t0 (TFun T0 T1) ->
     has_type ctx t1 T0 ->
     has_type ctx (tapp t0 t1) T1
-| ht_let : forall ctx i T bind body T',
-    has_type (update i T ctx) bind T ->
-    has_type (update i T ctx) body T' ->
-    has_type ctx (tlet i T bind body) T'
+| ht_let : forall ctx i T bind body T' (h: wf_ty T),
+    has_type (update i (exist _ T h) ctx) bind T ->
+    has_type (update i (exist _ T h) ctx) body T' ->
+    has_type ctx (tlet i T h bind body) T'
+| ht_fix : forall ctx i body T (h:wf_ty T),
+    has_type (update i (exist _ T h) ctx) body T ->
+    has_type ctx (tfix i T h body) T
 | ht_true : forall ctx,
     has_type ctx ttrue TBool
 | ht_false : forall ctx,
@@ -97,24 +114,66 @@ Inductive has_type : Context ty -> tm -> ty -> Prop :=
     has_type ctx t0 TBool ->
     has_type ctx t1 TBool ->
     has_type ctx (tbeq t0 t1) TBool
-| ht_left : forall ctx t0 TL TR,
+| ht_left : forall ctx t0 TL TR (h: wf_ty TR),
     has_type ctx t0 TL ->
-    has_type ctx (tleft t0 TR) (TSum TL TR)
-| ht_right : forall ctx t0 TL TR,
+    has_type ctx (tleft t0 TR h) (TSum TL TR)
+| ht_right : forall ctx t0 TL TR (h: wf_ty TL),
     has_type ctx t0 TR ->
-    has_type ctx (tright TL t0) (TSum TL TR)
+    has_type ctx (tright TL h t0) (TSum TL TR)
 | ht_case : forall ctx crit tl tr TL TR TO,
     has_type ctx crit (TSum TL TR) ->
     has_type ctx tl (TFun TL TO) ->
     has_type ctx tr (TFun TR TO) ->
     has_type ctx (tcase crit tl tr) TO
-| ht_field : forall ctx suty i,
-    rcd_field_ty rcd i = Some T ->
-    has_type (ht_field (TRcd tid suty rcd) i) (TFun (TRcd tid suty rcd) T)
+| ht_field : forall ctx i T0 T (h0: only_rcd T0) (h1: wf_ty T0),
+    rcd_field_ty T0 h0 h1 i = Some T ->
+    has_type ctx (tfield T0 h0 h1 i) (TFun T0 T)
 | ht_seq : forall ctx t0 t1 T0 T1,
-    has_type t0 T0 ->
-    has_type t1 T1 ->
-    has_type (tseq t0 t1) T1.
+    has_type ctx t0 T0 ->
+    has_type ctx t1 T1 ->
+    has_type ctx (tseq t0 t1) T1.
 
+Theorem has_type_well_formed:
+    forall ctx t T,
+        has_type ctx t T ->
+        wf_ty T.
+    intros t T ctx h.
+    
+    induction h; try (intros; subst; eauto 10; fail); intros; subst.
+    inversion IHh1; subst; eauto.
+    inversion IHh3; subst; eauto.
+    poses' (rcd_field_ty_well_formed _ _ _ _ _ H).
+    eauto.
+Qed.
+
+Inductive value : tm -> Prop :=
+    | vNone : value tnone
+    | vRcons : forall i t0 t1,
+                value t0 ->
+                value t1 ->
+                value (trcons i t0 t1)
+    | vInt : forall n,
+                value (tint n)
+    | vtrue : value ttrue
+    | vfalse : value tfalse
+    | vleft : forall t T wft,
+                value t ->
+                value (tleft t T wft)
+    | vright : forall T wft t,
+                value t ->
+                value (tright T wft t)
+    | vfield : forall T ort wft id,
+                value (tfield T ort wft id).
+
+Inductive step : tm -> tm -> Prop :=
+    | strcons0:
+        forall i t0 t0' t1,
+            step t0 t0' ->
+            step (trcons i t0 t1) (trcons i t0' t1)
+    | strcons1 :
+        forall i t0 t1 t1',
+            value t0 ->
+            step t1 t1' ->
+            step (trcons i t0 t1) (trcons i t0 t1') 
 
 End SSmtyP.
